upd

Computation.v
@@ -1,4 +1,4 @@
-Require Import List Arith Alphabet Language Lia.
+Require Import List Arith Alphabet Function Lia.
 
 Definition transition (state: Type) := state -> state + nat.
 
@@ -6,10 +6,6 @@ Section Computation.
   Context {state: Type}.
   Variable next: transition state.
   Variable encode_input: nat -> state.
-
-  Record decision_model :=
-    { dm_next: transition state; dm_enc: nat -> state }.
-  Definition dm_class := decision_model -> Prop.
 
   Inductive steps: state -> state -> Prop :=
   | stepsRefl: forall (s: state), steps s s
@@ -46,7 +42,7 @@ Section Computation.
   Qed.
 
   Lemma steps_eval:
-    forall (s s': state) (n: nat), steps s s' -> (decision s b <-> decision s' b).
+    forall (s s': state) (n: nat), steps s s' -> (eval s n <-> eval s' n).
   Proof.
     intros.
     induction H.
@@ -56,193 +52,67 @@ Section Computation.
       + inversion H; subst; rewrite H0 in H1.
         * discriminate.
         * inversion H1. auto.
-      + apply decisionStep with (s' := s''); auto.
+      + apply evalStep with (s' := s''); auto.
   Qed.
 
   Lemma steps_halts:
     forall (s s': state), steps s s' -> (halts s <-> halts s').
   Proof.
     intros.
-    split; intro.
-    - destruct H0.
-      + apply (steps_decision s s' true H) in H0. unfold halts. auto.
-      + apply (steps_decision s s' false H) in H0. unfold halts. auto.
-    - destruct H0.
-      + apply (steps_decision s s' true H) in H0. unfold halts. auto.
-      + apply (steps_decision s s' false H) in H0. unfold halts. auto.
+    split; intro; destruct H0;
+      apply (steps_eval s s' x H) in H0; unfold halts; eauto.
   Qed.
 
-  Lemma decision_unique: forall (s: state), ~(decision s true /\ decision s false).
-  Proof.
-    intros. intro.
-    destruct H.
-    assert (halts' s).
-    - apply halts_iff_halts'. unfold halts. auto.
-    - destruct H1.
-      induction H1.
-      + unfold halted in H1.
-        destruct H1.
-        * inversion H0; subst; rewrite H1 in H2; discriminate.
-        * inversion H; subst; rewrite H1 in H2; discriminate.
-      + inversion H; inversion H0; subst.
-        * rewrite H3 in H6. discriminate.
-        * rewrite H3 in H6. discriminate.
-        * rewrite H3 in H7. discriminate.
-        * rewrite H3 in H7. inversion H7. rewrite H1 in H3. inversion H3. subst.
-          apply IHruntime; auto.
-  Qed.
-
-  Definition decides (l: language) :=
-    forall (w: bitstr), halts (encode_input w) /\ (decision (encode_input w) true <-> l w).
-
-  Lemma language_unique: forall (l l': language), decides l -> decides l' -> l = l'.
+  Lemma eval_unique: forall (s: state) (n n': nat),
+    eval s n -> eval s n' -> n = n'.
   Proof.
     intros.
-    apply lang_extensionality.
-    intro. split; intro; unfold decides in *;
-    specialize H with w; specialize H0 with w; destruct H, H0; intuition.
+    assert (halts s).
+    - exists n. auto.
+    - rewrite halts_iff_halts' in H1.
+      destruct H1.
+      induction H1.
+      + destruct H1.
+        inversion H; inversion H0; subst.
+        * rewrite H2 in H5. inversion H5. auto.
+        * rewrite H2 in H5. discriminate.
+        * rewrite H2 in H6. discriminate.
+        * rewrite H2 in H1. discriminate.
+      + apply IHruntime; inversion H; inversion H0; subst.
+        * rewrite H1 in H3. discriminate.
+        * rewrite H6 in H3. discriminate.
+        * rewrite H3 in H7. discriminate.
+        * rewrite H1 in H3. inversion H3. subst. auto.
+        * rewrite H1 in H3. discriminate.
+        * rewrite H6 in H3. discriminate.
+        * rewrite H3 in H7. discriminate.
+        * rewrite H1 in H7. inversion H7. subst. auto.
   Qed.
 
-  Fixpoint simulate (s: state) (n: nat): option bool :=
+  Definition evaluates (f: function) :=
+    forall (n: nat), halts (encode_input n) /\ (eval (encode_input n) (f n)).
+
+  Lemma evaluation_unique: forall (f f': function), evaluates f -> evaluates f' -> f = f'.
+  Proof.
+    intros.
+    apply func_extensionality.
+    intro.
+    unfold evaluates in *.
+    specialize H with n.
+    specialize H0 with n.
+    destruct H, H0.
+    eapply eval_unique; eauto.
+  Qed.
+
+  Fixpoint simulate (s: state) (n: nat): option nat :=
     match n with
     | 0 => None
     | S m => match next s with
              | inl s' => simulate s' m
-             | inr b => Some b
+             | inr x => Some x
              end
     end.
 
   (* simulate correct *)
 End Computation.
 
-Section Simulation.
-  Definition dm_steps
-    {state: Type} (dm: @decision_model state) := steps (dm_next dm).
-  Definition dm_halts
-    {state: Type} (dm: @decision_model state) := halts (dm_next dm).
-  Definition dm_halted
-    {state: Type} (dm: @decision_model state) := halted (dm_next dm).
-  Definition dm_decision
-    {state: Type} (dm: @decision_model state) := decision (dm_next dm).
-  Definition dm_decides
-    {state: Type} (dm: @decision_model state) := decides (dm_next dm) (dm_enc dm).
-
-  Definition homomorphism
-    {state state': Type} (dm: @decision_model state) (dm': @decision_model state')
-    (h: state -> state') :=
-    (forall (w: bitstr), h (dm_enc dm w) = dm_enc dm' w) /\
-    (forall (s s': state), dm_steps dm s s' -> dm_steps dm' (h s) (h s')) /\
-    (forall (s: state), dm_halted dm s -> dm_halted dm' (h s)) /\
-    (forall (s: state) (b: bool), dm_next dm s = inr b -> dm_next dm' (h s) = inr b).
-
-  Local Lemma homomorphism_decision
-    {state state': Type} (dm: @decision_model state) (dm': @decision_model state')
-    (h: state -> state') (s: state) (b: bool):
-    homomorphism dm dm' h -> dm_decision dm s b -> dm_decision dm' (h s) b.
-  Proof.
-    intros.
-    destruct dm as [next enc].
-    destruct dm' as [next' enc'].
-    unfold homomorphism in H.
-    destruct H. destruct H1. destruct H2.
-    unfold dm_decision in *.
-    unfold dm_halted in *.
-    unfold dm_steps in *.
-    simpl in *.
-    induction H0.
-    - apply H3 in H0.
-      repeat econstructor. auto.
-    - assert (steps next s s').
-      + repeat econstructor. auto.
-      + apply H1 in H5.
-        rewrite (steps_decision next' (h s) (h s') b H5).
-        auto.
-  Qed.
-
-  Lemma homomorphism_decides
-    {state state': Type} (dm: @decision_model state) (dm': @decision_model state')
-    (h: state -> state') (l: language):
-    homomorphism dm dm' h -> dm_decides dm l -> dm_decides dm' l.
-  Proof.
-    intros.
-    destruct dm as [next enc].
-    destruct dm' as [next' enc'].
-    unfold dm_decides in *.
-    remember H as He. clear HeqHe.
-    destruct He as [Henc H']. clear H'.
-    simpl in *.
-    intro.
-    specialize Henc with w.
-    split.
-    - unfold decides in H0.
-      specialize H0 with w.
-      destruct H0.
-      unfold halts in *.
-      destruct H0.
-      + left.
-        remember H as He. clear HeqHe.
-        apply homomorphism_decision with (s := enc w) (b := true) in H; auto.
-        unfold dm_decision in H. simpl in H.
-        rewrite <- Henc.
-        auto.
-      + right.
-        apply homomorphism_decision with (s := enc w) (b := false) in H; auto.
-        unfold dm_decision in H. simpl in H.
-        rewrite <- Henc.
-        auto.
-    - unfold decides in H0.
-      specialize H0 with w.
-      destruct H0.
-      rewrite <- H1. clear H1.
-      split.
-      + intro.
-        destruct H0; auto.
-        apply homomorphism_decision with (s := enc w) (b := false) in H.
-        unfold dm_decision in H; simpl in H; intros.
-        * rewrite Henc in H.
-          exfalso.
-          apply (decision_unique next' (enc' w)).
-          intuition.
-        * unfold dm_decision. simpl. auto.
-      + intro.
-        apply homomorphism_decision with (s := enc w) (b := true) in H;
-        unfold dm_decision in H; simpl in H; intros.
-        * rewrite <- Henc. auto.
-        * unfold dm_decision. simpl.
-          destruct H0 eqn: Ha; auto.
-  Qed.
-
-  Lemma homomorphism_compose
-    {state state' state'': Type}
-    (dm: @decision_model state) (dm': @decision_model state') (dm'': @decision_model state'')
-    (h: state -> state') (h': state' -> state''):
-    homomorphism dm dm' h -> homomorphism dm' dm'' h' ->
-    homomorphism dm dm'' (fun x => h' (h x)).
-  Proof.
-    intros.
-    destruct dm as [next enc].
-    destruct dm' as [next' enc'].
-    destruct dm'' as [next'' enc''].
-    unfold homomorphism in *.
-    destruct H. destruct H1. destruct H2.
-    destruct H0. destruct H4. destruct H5.
-    unfold dm_decision in *.
-    unfold dm_halted in *.
-    unfold dm_steps in *.
-    simpl in *.
-    split; try split; try split; intros.
-    - rewrite <- H0. rewrite <- H. auto.
-    - apply H4. apply H1. auto.
-    - apply H5. apply H2. auto.
-    - apply H6. apply H3. auto.
-  Qed.
-
-  (*
-     Lemma homomorphism identity
-     Definition class_subset
-     Lemma subset_refl
-     Lemma subset_transitive
-     Lemma subset_subset
-   *)
-
-End Simulation.
