Util.v
@@ -1,5 +1,149 @@
-Require Import Arith Language Lia.
+Require Import Arith Function Lia List IMP.
+Import ListNotations.
 
 
 Definition isomorphism {A B: Type} (f: A -> B) (finv: B -> A) :=
   (forall x, finv (f x) = x) /\ (forall x, f (finv x) = x).
+
+
+Fixpoint str_S (w: bitstr) :=
+  match w with
+  | nil => cons false nil
+  | cons b rest => match b with
+                   | false => cons true rest
+                   | true => cons false (str_S rest)
+                   end
+  end.
+
+Fixpoint str_P (w: bitstr): option bitstr :=
+  match w with
+  | nil => None
+  | cons b rest => Some (match b with
+                         | true => cons false rest
+                         | false => match (str_P rest) with
+                                    | None => nil
+                                    | Some r => cons true r
+                                    end
+                         end)
+  end.
+
+Lemma str_P_correct: forall w, str_P (str_S w) = Some w.
+Proof.
+  intros.
+  induction w; auto.
+  unfold str_S. fold str_S.
+  destruct a.
+  - unfold str_P. fold str_P.
+    rewrite IHw. auto.
+  - unfold str_P. fold str_P.
+    auto.
+Qed.
+
+Fixpoint nat_to_str (n: nat) :=
+  match n with
+  | 0 => nil
+  | S m => str_S (nat_to_str m)
+  end.
+
+Lemma nat_to_str_inj (n n': nat): nat_to_str n = nat_to_str n' -> n = n'.
+Proof.
+
+Admitted.
+
+
+Fixpoint str_to_nat' (w: bitstr) :=
+  match w with
+  | nil => 1
+  | cons b rest => (if b then 1 else 0) + 2 * (str_to_nat' rest)
+  end.
+
+Definition str_to_nat (w: bitstr) := (str_to_nat' w) - 1.
+
+Lemma nat_to_str'_pos: forall w, str_to_nat' w > 0.
+Proof.
+  intros.
+  induction w; auto.
+  unfold str_to_nat'. fold str_to_nat'. lia.
+Qed.
+
+Lemma S_nat_to_str': forall w, S (str_to_nat' w) = str_to_nat' (str_S w).
+Proof.
+  intros.
+  induction w; auto.
+  destruct a;
+  unfold str_S; fold str_S;
+  unfold str_to_nat'; fold str_to_nat'.
+  - rewrite <- IHw. lia.
+  - lia.
+Qed.
+
+Lemma S_nat_to_str: forall w, S (str_to_nat w) = str_to_nat (str_S w).
+Proof.
+  unfold str_to_nat.
+  intro.
+  rewrite <- S_nat_to_str'.
+  remember (nat_to_str'_pos w).
+  lia.
+Qed.
+
+
+Lemma nat_str_iso: isomorphism nat_to_str str_to_nat.
+Proof.
+
+Admitted.
+
+
+Fixpoint read_n (w: bitstr): nat * bitstr :=
+  match w with
+  | nil => (0, nil)
+  | false :: w' => (0, w')
+  | true :: w' => let (n, w'') := read_n w' in (n+1, w'')
+  end.
+
+Definition read_instr (w: bitstr): L_instr * bitstr :=
+  match w with
+  | false :: false :: false :: false :: w' => (NOP, w')
+  | false :: false :: false :: true :: w' =>
+      let (rt, w'') := read_n w' in let (n, w''') := read_n w'' in (LDI rt n, w''')
+  | false :: false :: true :: false :: w' =>
+      let (rt, w'') := read_n w' in let (ra, w''') := read_n w'' in
+      let (rb, w'''') := read_n w''' in (ADD rt ra rb, w'''')
+  | false :: false :: true :: true :: w' =>
+      let (rt, w'') := read_n w' in let (ra, w''') := read_n w'' in
+      let (rb, w'''') := read_n w''' in (SUB rt ra rb, w'''')
+  | false :: true :: true :: true :: w' =>
+      let (rt, w'') := read_n w' in let (ra, w''') := read_n w'' in
+      let (rb, w'''') := read_n w''' in (MUL rt ra rb, w'''')
+  | false :: true :: true :: false :: w' =>
+      let (rt, w'') := read_n w' in let (ra, w''') := read_n w'' in
+      let (rb, w'''') := read_n w''' in (DIV rt ra rb, w'''')
+  | false :: true :: false :: false :: w' =>
+      let (rt, w'') := read_n w' in let (ra, w''') := read_n w'' in
+      let (rb, w'''') := read_n w''' in (MOD rt ra rb, w'''')
+  | false :: true :: false :: true :: w' =>
+      let (rt, w'') := read_n w' in let (ra, w''') := read_n w'' in
+      let (rb, w'''') := read_n w''' in (EQ rt ra rb, w'''')
+  | true :: true :: true :: false :: w' =>
+      let (i, w'') := read_n w' in let (rc, w''') := read_n w'' in (JNE i rc, w''')
+  | true :: false :: true :: false :: w' =>
+      let (i, w'') := read_n w' in let (rc, w''') := read_n w'' in (JRNE i rc, w''')
+  | true :: false :: false :: false :: w' =>
+      let (i, w'') := read_n w' in let (rc, w''') := read_n w'' in (JBNE i rc, w''')
+  | true :: true :: false :: false :: w' =>
+      let (rt, w'') := read_n w' in (RET rt, w'')
+  | _ => (NOP, nil)
+  end.
+
+
+
+
+Fixpoint str_to_limp (w: bitstr) (n: nat): L_prog :=
+  match n with
+  | 0 => nil
+  | S m => match read_instr w with
+           | (instr, nil) => [instr]
+           | (instr, w') => instr :: str_to_limp w' m
+           end
+  end.
+
+Definition nat_to_limp (n: nat) := str_to_limp (nat_to_str n) (length (nat_to_str n)).
