Halt.v
@@ -1,0 +1,13 @@
+Require Import Arith Function Computation Lia List IMP Util.
+
+Print halts.
+
+
+Definition HALT_0 (f: function) :=
+  forall n, f n < 2 /\
+  (f n = 1 <-> halts (L_next (nat_to_limp n)) L_initial).
+
+
+Definition HALT_ALL (f: function) :=
+  forall n, f n < 2 /\
+  (f n = 1 <-> forall m, halts (L_next (nat_to_limp n)) (L_input_initial m)).
