IMP.v
@@ -1,0 +1,55 @@
+Require Import Arith List Function Computation.
+Import ListNotations.
+
+Definition reg_map := nat -> nat.
+Definition empty_reg_map (n: nat) := 0.
+Definition upd_reg_map (m: reg_map) (i x j: nat) :=
+  if Nat.eq_dec i j then x else m j.
+
+
+Inductive L_instr :=
+  | NOP
+  | LDI (rt n: nat)
+  | ADD (rt ra rb: nat)
+  | SUB (rt ra rb: nat)
+  | MUL (rt ra rb: nat)
+  | DIV (rt ra rb: nat)
+  | MOD (rt ra rb: nat)
+  | EQ (rt ra rb: nat)
+  | JNE (i rc: nat)
+  | JRNE (i rc: nat)
+  | JBNE (i rc: nat)
+  | RET (ra: nat)
+.
+
+Definition L_prog := list L_instr.
+
+Record L_state := { l_ip: nat; l_mem: reg_map }.
+Definition L_initial := Build_L_state 0 empty_reg_map.
+Definition L_input_initial (x: nat) := Build_L_state 0 (upd_reg_map empty_reg_map 0 x).
+
+Definition eq (n m: nat) :=
+  if Nat.eq_dec n m then 1 else 0.
+
+Definition L_next (p: L_prog) (st: L_state): L_state + nat :=
+  let (ip, mem) := st in
+  match nth ip p (RET 0) with
+  | NOP => inl (Build_L_state (ip+1) mem)
+  | LDI rt n => inl (Build_L_state (ip+1) (upd_reg_map mem rt n))
+  | ADD rt ra rb => inl (Build_L_state (ip+1) (upd_reg_map mem rt (mem ra + mem rb)))
+  | SUB rt ra rb => inl (Build_L_state (ip+1) (upd_reg_map mem rt (mem ra - mem rb)))
+  | MUL rt ra rb => inl (Build_L_state (ip+1) (upd_reg_map mem rt (mem ra * mem rb)))
+  | DIV rt ra rb => inl (Build_L_state (ip+1) (upd_reg_map mem rt (mem ra / mem rb)))
+  | MOD rt ra rb => inl (Build_L_state (ip+1) (upd_reg_map mem rt (mem ra mod mem rb)))
+  | EQ rt ra rb => inl (Build_L_state (ip+1) (upd_reg_map mem rt (eq (mem ra) (mem rb))))
+  | JNE i rc =>
+      inl (Build_L_state (if mem rc then i else ip+1) mem)
+  | JRNE i rc =>
+      inl (Build_L_state (if mem rc then ip+i else ip+1) mem)
+  | JBNE i rc =>
+      inl (Build_L_state (if mem rc then ip-i else ip+1) mem)
+  | RET ra => inr (mem ra)
+  end.
+
+
+
